keep track of consumed map entries (currently, only internally)

share/pulse/examples/dice/cbor/CDDL.Spec.MapGroupGen.fst
@@ -268,14 +268,65 @@ let is_sublist_of_prefix
 = List.Tot.append_l_nil l1;
   is_sublist_of_append_left_intro l1 [] l2
 
+module FE = FStar.FunctionalExtensionality
+
+let ghost_map (key value: Type) : Type =
+  FE.restricted_g_t key (fun _ -> option value)
+
+let ghost_map_mem (#key #value: Type) (kv: (key & value)) (f: ghost_map key value) : Tot prop =
+  f (fst kv) == Some (snd kv)
+
+let ghost_map_feq (#key #value: Type) (f1 f2: ghost_map key value) : Tot prop =
+  FE.feq_g f1 f2
+
+let ghost_map_feq_eq (#key #value: Type) (f1 f2: ghost_map key value) : Lemma
+  (ensures (ghost_map_feq f1 f2 <==> f1 == f2))
+  [SMTPat (ghost_map_feq f1 f2)]
+= ()
+
+let ghost_map_equiv_intro
+  (#key #value: Type) (f1 f2: ghost_map key value)
+  (prf12: (x: (key * value)) -> Lemma (requires ghost_map_mem x f1) (ensures ghost_map_mem x f2))
+  (prf21: (x: (key * value)) -> Lemma (requires ghost_map_mem x f2) (ensures ghost_map_mem x f1))
+: Lemma
+  (f1 == f2)
+= let prf x y : Lemma (f1 x == Some y <==> f2 x == Some y) =
+    let xy = (x, y) in
+    Classical.move_requires prf12 xy;
+    Classical.move_requires prf21 xy;
+    assert (ghost_map_mem xy f1 <==> ghost_map_mem xy f2)
+  in
+  Classical.forall_intro_2 prf;
+  assert (FE.feq_g f1 f2)
+
+
+let ghost_map_equiv_intro'
+  (#key #value: Type) (f1 f2: ghost_map key value)
+  (prf: (x: (key * value)) -> Lemma (ghost_map_mem x f1 <==> ghost_map_mem x f2))
+: Lemma
+  (f1 == f2)
+= ghost_map_equiv_intro f1 f2 (fun x -> prf x) (fun x -> prf x)
+
+#restart-solver
+let ghost_map_equiv (#key #value: Type) (f1 f2: ghost_map key value) : Lemma
+  (requires (forall kv . ghost_map_mem kv f1 <==> ghost_map_mem kv f2))
+  (ensures f1 == f2)
+= ghost_map_equiv_intro' f1 f2 (fun _ -> ())
+
+let ghost_map_defined (#key #value: Type) (k: key) (f: ghost_map key value) : Tot prop =
+  Some? (f k)
+
+let ghost_map_disjoint (#key #value1 #value2: Type) (f1: ghost_map key value1) (f2: ghost_map key value2) : Tot prop =
+  (forall k . ~ (ghost_map_defined k f1 /\ ghost_map_defined k f2))
+
 let map_group_item_post
   (l: list (Cbor.raw_data_item & Cbor.raw_data_item))
-  (l': (list (Cbor.raw_data_item & Cbor.raw_data_item) & list (Cbor.raw_data_item & Cbor.raw_data_item)))
+  (l': (ghost_map Cbor.raw_data_item Cbor.raw_data_item & list (Cbor.raw_data_item & Cbor.raw_data_item)))
 : Tot prop
 =
-        (snd l' `is_sublist_of` l) /\
-        List.Tot.length (fst l') + List.Tot.length (snd l') == List.Tot.length l /\
-        (forall x . (List.Tot.memP x (fst l') \/ List.Tot.memP x (snd l')) <==> List.Tot.memP x l)
+  (snd l' `is_sublist_of` l) /\
+  (forall x . ~ (ghost_map_defined x (fst l') /\ List.Tot.memP x (List.Tot.map fst (snd l')))) /\
+  (forall x . (ghost_map_mem x (fst l') \/ List.Tot.memP x (snd l')) <==> List.Tot.memP x l)
 
 let rec list_memP_extract
   (#t: Type)
@@ -396,49 +447,125 @@ let list_ghost_assoc_memP_strong'
   (ensures (forall k v . Cbor.list_ghost_assoc k l == Some v <==> List.Tot.memP (k, v) l))
 = Classical.forall_intro_2 (fun k v -> Classical.move_requires (list_ghost_assoc_memP_strong k v) l)
 
+let rec list_ghost_assoc_memP
+  (#key #value: Type)
+  (k: key)
+  (l: list (key & value))
+: Lemma
+  (ensures (Some? (Cbor.list_ghost_assoc k l) <==> List.Tot.memP k (List.Tot.map fst l)))
+  (decreases l)
+= match l with
+  | [] -> ()
+  | _ :: q -> list_ghost_assoc_memP k q
+
 #restart-solver
 let map_group_item_post_prop
   (l: cbor_map)
-  (l': (list (Cbor.raw_data_item & Cbor.raw_data_item) & list (Cbor.raw_data_item & Cbor.raw_data_item)))
+  (l': (ghost_map Cbor.raw_data_item Cbor.raw_data_item & list (Cbor.raw_data_item & Cbor.raw_data_item)))
 : Lemma
   (requires (map_group_item_post l l'))
   (ensures (
-    List.Tot.no_repeats_p (List.Tot.map fst (fst l' `List.Tot.append` snd l')) /\
-    List.Tot.no_repeats_p (List.Tot.map fst (fst l')) /\
     List.Tot.no_repeats_p (List.Tot.map fst (snd l')) /\
-    (forall x . Cbor.list_ghost_assoc x (fst l' `List.Tot.append` snd l') == Cbor.list_ghost_assoc x l)
+    (forall xy . ~ (ghost_map_mem xy (fst l') /\ List.Tot.memP xy (snd l'))) /\
+    (forall x . Cbor.list_ghost_assoc x l == begin match fst l' x with
+    | Some y -> Some y
+    | None -> Cbor.list_ghost_assoc x (snd l')
+    end) /\
+    (forall x . Cbor.list_ghost_assoc x l == begin match Cbor.list_ghost_assoc x (snd l') with
+    | Some y -> Some y
+    | None -> fst l' x
+    end)
   ))
   [SMTPat (map_group_item_post l l')]
-=
-  Classical.forall_intro (List.Tot.append_memP (fst l') (snd l'));
-  Classical.forall_intro (list_memP_map fst l);
-  Classical.forall_intro (list_memP_map fst (fst l' `List.Tot.append` snd l'));
-  List.Tot.map_append fst (fst l') (snd l');
-  list_memP_equiv_no_repeats (List.Tot.map fst l) (List.Tot.map fst (fst l' `List.Tot.append` snd l'));
-  assert (List.Tot.no_repeats_p (List.Tot.map fst (fst l' `List.Tot.append` snd l')));
-  list_no_repeats_p_is_sublist_of (List.Tot.map fst (fst l')) (List.Tot.map fst (fst l' `List.Tot.append` snd l'));
-  assert (List.Tot.no_repeats_p (List.Tot.map fst (fst l')));
-  list_no_repeats_p_is_sublist_of (List.Tot.map fst (snd l')) (List.Tot.map fst (fst l' `List.Tot.append` snd l'));
-  assert (List.Tot.no_repeats_p (List.Tot.map fst (snd l')));
-  let prf x y : Lemma
-    (Cbor.list_ghost_assoc x (fst l' `List.Tot.append` snd l') == Some y <==> Cbor.list_ghost_assoc x l == Some y)
-  = list_ghost_assoc_memP_strong' l ();
-    list_ghost_assoc_memP_strong' (fst l' `List.Tot.append` snd l') ();
-    List.Tot.append_memP (fst l') (snd l') (x, y)
+= 
+  list_map_is_sublist_of fst (snd l') l;
+  list_no_repeats_p_is_sublist_of (List.Tot.map fst (snd l')) (List.Tot.map fst l);
+  assert ( 
+    List.Tot.no_repeats_p (List.Tot.map fst (snd l'))
+  );
+  Classical.forall_intro (fun x -> List.Tot.memP_map_intro fst x (snd l'));
+  assert
+    (forall xy . ~ (ghost_map_mem xy (fst l') /\ List.Tot.memP xy (snd l')));
+  let prf xv : Lemma
+    (let (x, v) = xv in Cbor.list_ghost_assoc x l == Some v <==> (ghost_map_mem (x, v) (fst l') \/ (Cbor.list_ghost_assoc x (snd l') == Some v /\ ~ (ghost_map_defined x (fst l')))))
+  = let (x, v) = xv in
+    list_ghost_assoc_memP x (snd l');
+    list_ghost_assoc_memP_strong x v l;
+    list_ghost_assoc_memP_strong x v (snd l')
   in
-  let prf x : Lemma
-    (Cbor.list_ghost_assoc x (fst l' `List.Tot.append` snd l') == Cbor.list_ghost_assoc x l)
-  = Classical.forall_intro (prf x)
+  let prf2 x : Lemma (Cbor.list_ghost_assoc x l == begin match fst l' x with
+    | Some y -> Some y
+    | None -> Cbor.list_ghost_assoc x (snd l')
+  end) =
+    match Cbor.list_ghost_assoc x l with
+    | Some v -> prf (x, v)
+    | _ -> match fst l' x with
+          | Some v -> prf (x, v)
+          | _ -> match Cbor.list_ghost_assoc x (snd l') with
+                 | Some v -> prf (x, v)
+                 | _ -> ()
   in
-  Classical.forall_intro prf;
-  assert (forall x . Cbor.list_ghost_assoc x (fst l' `List.Tot.append` snd l') == Cbor.list_ghost_assoc x l)
+  Classical.forall_intro prf2;
+  assert (forall x . Cbor.list_ghost_assoc x l == begin match fst l' x with
+    | Some y -> Some y
+    | None -> Cbor.list_ghost_assoc x (snd l')
+  end);
+  let prf3 x : Lemma (Cbor.list_ghost_assoc x l == begin match Cbor.list_ghost_assoc x (snd l') with
+    | Some y -> Some y
+    | None -> fst l' x
+  end) =
+    match Cbor.list_ghost_assoc x (snd l') with
+          | Some v ->
+            list_ghost_assoc_memP x (snd l');
+            assert (~ (ghost_map_defined x (fst l'))); prf (x, v)
+          | _ -> match fst l' x with
+                 | Some v -> prf (x, v)
+                 | _ -> ()
+  in
+  Classical.forall_intro prf3;
+  assert (forall x . Cbor.list_ghost_assoc x l == begin match Cbor.list_ghost_assoc x (snd l') with
+    | Some y -> Some y
+    | None -> fst l' x
+  end)
+
+let ghost_map_empty (#key #value: Type) : Tot (ghost_map key value) =
+  FE.on_dom_g _ (fun _ -> None)
+
+let ghost_map_singleton (#key #value: Type) (k: key) (v: value) : Tot (ghost_map key value) =
+  FE.on_dom_g _ (fun k' ->
+    if FStar.StrongExcludedMiddle.strong_excluded_middle (k == k')
+    then Some v
+    else None
+  )
+
+let ghost_map_union (#key #value: Type) (m1 m2: ghost_map key value) : Tot (ghost_map key value) =
+  FE.on_dom_g _ (fun k' ->
+    let res1 = m1 k' in
+    if Some? res1
+    then res1
+    else m2 k'
+  )
+
+let ghost_map_disjoint_mem_union (#key #value: Type) (m1 m2: ghost_map key value) (xv: (key & value)) : Lemma
+  (requires ghost_map_disjoint m1 m2)
+  (ensures ghost_map_mem xv (m1 `ghost_map_union` m2) <==> ghost_map_mem xv m1 \/ ghost_map_mem xv m2)
+= ()
+
+let ghost_map_disjoint_mem_union' (#key #value: Type) (m1 m2: ghost_map key value) (_: squash (ghost_map_disjoint m1 m2)) : Lemma
+  (ensures forall xv . ghost_map_mem xv (m1 `ghost_map_union` m2) <==> ghost_map_mem xv m1 \/ ghost_map_mem xv m2)
+= ()
+
+let ghost_map_disjoint_union (#key #value: Type) (m1 m2: ghost_map key value) : Lemma
+  (requires ghost_map_disjoint m1 m2)
+  (ensures m1 `ghost_map_union` m2 == m2 `ghost_map_union` m1)
+= assert ((m1 `ghost_map_union` m2) `FE.feq_g` (m2 `ghost_map_union` m1))
 
 let map_group_post
   (l: list (Cbor.raw_data_item & Cbor.raw_data_item))
-  (res: FStar.GSet.set (list (Cbor.raw_data_item & Cbor.raw_data_item) & list (Cbor.raw_data_item & Cbor.raw_data_item)))
+  (res: FStar.GSet.set _)
 : Tot prop
 =
-      forall (l': (list (Cbor.raw_data_item & Cbor.raw_data_item) & list (Cbor.raw_data_item & Cbor.raw_data_item))) .
+      forall l' .
       FStar.GSet.mem l' res ==>  map_group_item_post l l'
 
 let cbor_map_is_sublist_of
@@ -451,12 +578,10 @@ let cbor_map_is_sublist_of
   [SMTPat (l1 `is_sublist_of` l2)]
 = Classical.move_requires (list_map_is_sublist_of fst l1) l2
 
-module FE = FStar.FunctionalExtensionality
-
 let map_group_codom
   (l: cbor_map)
 : Tot Type0
-= (res: FStar.GSet.set (list (Cbor.raw_data_item & Cbor.raw_data_item) & list (Cbor.raw_data_item & Cbor.raw_data_item)) {
+= (res: FStar.GSet.set _ {
       map_group_post l res
   })
 
@@ -469,18 +594,18 @@ let map_group_always_false : map_group =
   FE.on_dom_g cbor_map #map_group_codom
     (fun _ -> FStar.GSet.empty)
 
-let map_group_end : map_group =
-  FE.on_dom_g cbor_map #map_group_codom
-    (fun l -> if Nil? l then FStar.GSet.singleton ([], l) else FStar.GSet.empty)
-
 let map_group_nop : map_group =
   FE.on_dom_g cbor_map #map_group_codom
-    (fun l -> FStar.GSet.singleton ([], l))
+    (fun l -> FStar.GSet.singleton (ghost_map_empty, l))
 
-let map_group_match_item_witness_pred (key value: typ) (l: list (Cbor.raw_data_item & Cbor.raw_data_item)) (l': (list (Cbor.raw_data_item & Cbor.raw_data_item) & list (Cbor.raw_data_item & Cbor.raw_data_item))) (x: (list (Cbor.raw_data_item & Cbor.raw_data_item) & (Cbor.raw_data_item & Cbor.raw_data_item) & list (Cbor.raw_data_item & Cbor.raw_data_item))) : Tot prop =
+let map_group_end : map_group =
+  FE.on_dom_g cbor_map #map_group_codom
+    (fun l -> if Nil? l then map_group_nop l else map_group_always_false l)
+
+let map_group_match_item_witness_pred (key value: typ) (l: list (Cbor.raw_data_item & Cbor.raw_data_item)) (l': (ghost_map Cbor.raw_data_item Cbor.raw_data_item & list (Cbor.raw_data_item & Cbor.raw_data_item))) (x: (list (Cbor.raw_data_item & Cbor.raw_data_item) & (Cbor.raw_data_item & Cbor.raw_data_item) & list (Cbor.raw_data_item & Cbor.raw_data_item))) : Tot prop =
   let (l1, (k, v), l2) = x in
       l == l1 `List.Tot.append` ((k, v) :: l2) /\
-      fst l' == [k, v] /\
+      fst l' == ghost_map_singleton k v /\
       snd l' == l1 `List.Tot.append` l2 /\
       key k /\
       value v
@@ -509,12 +634,15 @@ let map_group_match_item_witness_pred_is_sublist_of (key value: typ) (l: cbor_ma
   let (l1, kv, l2) = x in
   list_remove_is_sublist_of l1 kv l2;
   assert (snd l' `is_sublist_of` l);
-  List.Tot.append_assoc l1 [kv] l2;
-  List.Tot.append_length l1 l2;
-  assert (List.Tot.length (fst l') + List.Tot.length (snd l') == List.Tot.length l);
   Classical.forall_intro (List.Tot.append_memP l1 (kv :: l2));
   Classical.forall_intro (List.Tot.append_memP l1 l2);
-  assert (forall x . (List.Tot.memP x (fst l') \/ List.Tot.memP x (snd l')) <==> List.Tot.memP x l)
+  assert (forall x . (ghost_map_mem x (fst l') \/ List.Tot.memP x (snd l')) <==> List.Tot.memP x l);
+  List.Tot.map_append fst l1 (kv :: l2);
+  List.Tot.map_append fst l1 l2;
+  Classical.forall_intro (list_memP_map fst (l1 `List.Tot.append` (kv :: l2)));
+  Classical.forall_intro (list_memP_map fst (l1 `List.Tot.append` l2));
+  List.Tot.no_repeats_p_append_permut [] [] (List.Tot.map fst l1) [fst kv] (List.Tot.map fst l2);
+  assert (forall x . ~ (ghost_map_defined x (fst l') /\ List.Tot.memP x (List.Tot.map fst (snd l'))))
 
 let map_group_match_item_comprehend
   (key value: typ)
@@ -552,7 +680,7 @@ let map_group_match_item_alt (key value: typ) (l: cbor_map) : GTot _ =
   match list_filter_and_extract (FStar.Ghost.Pull.pull (matches_map_group_entry key value)) l with
   | None -> FStar.GSet.empty
   | Some (l1, x, l2) ->
-    FStar.GSet.union (FStar.GSet.singleton ([x], l1 `List.Tot.append` l2)) (gset_map (map_group_match_item_alt_r (l1 `List.Tot.append` [x])) (map_group_match_item key value l2))
+    FStar.GSet.union (FStar.GSet.singleton (ghost_map_singleton (fst x) (snd x), l1 `List.Tot.append` l2)) (gset_map (map_group_match_item_alt_r (l1 `List.Tot.append` [x])) (map_group_match_item key value l2))
 
 #push-options "--z3rlimit 32"
 
@@ -564,7 +692,7 @@ let map_group_match_item_alt_map_group_match_item
 = if FStar.GSet.mem l' (map_group_match_item_alt key value l)
   then begin
     let Some (l1, x, l2) = list_filter_and_extract (FStar.Ghost.Pull.pull (matches_map_group_entry key value)) l in
-    if FStar.StrongExcludedMiddle.strong_excluded_middle (l' == ([x], l1 `List.Tot.append` l2))
+    if FStar.StrongExcludedMiddle.strong_excluded_middle (l' == (ghost_map_singleton (fst x) (snd x), l1 `List.Tot.append` l2))
     then assert (map_group_match_item_witness_pred key value l l' (l1, x, l2))
     else begin
       let l2' = FStar.IndefiniteDescription.indefinite_description_ghost _ (gset_map_witness_pred (map_group_match_item_alt_r (l1 `List.Tot.append` [x])) (map_group_match_item key value l2) l') in
@@ -644,9 +772,10 @@ let map_group_match_item_map_group_match_item_alt
       let lp = list_extract_prefix (ll `List.Tot.append` [x]) lr ll' (x' :: lr') in
       List.Tot.append_assoc (ll `List.Tot.append` [x]) lp (x' :: lr');
       List.Tot.append_inv_head (ll `List.Tot.append` [x]) lr (lp `List.Tot.append` (x' :: lr'));
-      assert (map_group_match_item_witness_pred key value lr ([x'], lp `List.Tot.append` lr') (lp, x', lr'));
+      let mx' = ghost_map_singleton (fst x') (snd x') in
+      assert (map_group_match_item_witness_pred key value lr (mx', lp `List.Tot.append` lr') (lp, x', lr'));
       List.Tot.append_assoc (ll `List.Tot.append` [x]) lp lr';
-      assert (gset_map_witness_pred (map_group_match_item_alt_r (ll `List.Tot.append` [x])) (map_group_match_item key value lr) l' ([x'], lp `List.Tot.append` lr'))
+      assert (gset_map_witness_pred (map_group_match_item_alt_r (ll `List.Tot.append` [x])) (map_group_match_item key value lr) l' (mx', lp `List.Tot.append` lr'))
     end
   end
 
@@ -685,35 +814,67 @@ let map_group_cut (cut: typ) (m: map_group) : map_group =
   FE.on_dom_g cbor_map #map_group_codom (fun l -> 
     if List.Tot.for_all (notp (FStar.Ghost.Pull.pull (matches_map_group_entry cut any))) l
     then m l
-    else FStar.GSet.empty
+    else map_group_always_false l
   )
 
 let map_group_concat_witness_pred
   (m1 m2: map_group)
   (l: cbor_map)
-  (l': (list (Cbor.raw_data_item & Cbor.raw_data_item) & list (Cbor.raw_data_item & Cbor.raw_data_item)))
-  (l1l2: (list (Cbor.raw_data_item & Cbor.raw_data_item) & list (Cbor.raw_data_item & Cbor.raw_data_item)) & (list (Cbor.raw_data_item & Cbor.raw_data_item) & list (Cbor.raw_data_item & Cbor.raw_data_item)))
+  (l': (ghost_map Cbor.raw_data_item Cbor.raw_data_item & list (Cbor.raw_data_item & Cbor.raw_data_item)))
+  (l1l2: (ghost_map Cbor.raw_data_item Cbor.raw_data_item & list (Cbor.raw_data_item & Cbor.raw_data_item)) & (ghost_map Cbor.raw_data_item Cbor.raw_data_item & list (Cbor.raw_data_item & Cbor.raw_data_item)))
 : Tot prop
 = let (l1, l2) = l1l2 in
   FStar.GSet.mem l1 (m1 l) /\
   FStar.GSet.mem l2 (m2 (snd l1)) /\
-  l' == (fst l1 `List.Tot.append` fst l2, snd l2)
+  fst l' `ghost_map_feq` (fst l1 `ghost_map_union` fst l2) /\
+  snd l' == snd l2
 
+let ghost_map_disjoint_union_included_in_list
+  (#key #value: Type)
+  (f1 f2: ghost_map key value)
+  (l: list (key & value))
+: Lemma
+  (requires (
+    (forall x . ~ (ghost_map_defined x f1 /\ List.Tot.memP x (List.Tot.map fst l))) /\
+    (forall x . ghost_map_mem x f2 ==> List.Tot.memP x l)
+  ))
+  (ensures (
+    ghost_map_disjoint f1 f2
+  ))
+= let prf x : Lemma (ghost_map_defined x f2 ==> List.Tot.memP x (List.Tot.map fst l))
+  = if Some? (f2 x)
+    then begin
+      let Some v = f2 x in
+      List.Tot.memP_map_intro fst (x, v) l
+    end
+  in
+  Classical.forall_intro prf
+
+#push-options "--z3rlimit 16"
+
+#restart-solver
 let map_group_concat_witness_pred_correct
   (m1 m2: map_group)
   (l: cbor_map)
-  (l': (list (Cbor.raw_data_item & Cbor.raw_data_item) & list (Cbor.raw_data_item & Cbor.raw_data_item)))
-  (l1l2: (list (Cbor.raw_data_item & Cbor.raw_data_item) & list (Cbor.raw_data_item & Cbor.raw_data_item)) & (list (Cbor.raw_data_item & Cbor.raw_data_item) & list (Cbor.raw_data_item & Cbor.raw_data_item)))
+  (l': (ghost_map Cbor.raw_data_item Cbor.raw_data_item & list (Cbor.raw_data_item & Cbor.raw_data_item)))
+  (l1l2: (ghost_map Cbor.raw_data_item Cbor.raw_data_item & list (Cbor.raw_data_item & Cbor.raw_data_item)) & (ghost_map Cbor.raw_data_item Cbor.raw_data_item & list (Cbor.raw_data_item & Cbor.raw_data_item)))
 : Lemma
   (requires map_group_concat_witness_pred m1 m2 l l' l1l2)
-  (ensures map_group_item_post l l')
+  (ensures map_group_item_post l l' /\
+    fst (fst l1l2) `ghost_map_disjoint` fst (snd l1l2))
   [SMTPat (map_group_concat_witness_pred m1 m2 l l' l1l2)]
 = let (l1, l2) = l1l2 in
   assert (snd l' `is_sublist_of` l);
-  List.Tot.append_length (fst l1) (fst l2);
-  assert (List.Tot.length (fst l') + List.Tot.length (snd l') == List.Tot.length l);
-  Classical.forall_intro (List.Tot.append_memP (fst l1) (fst l2));
-  assert (forall x . (List.Tot.memP x (fst l') \/ List.Tot.memP x (snd l')) <==> List.Tot.memP x l)
+  ghost_map_disjoint_union_included_in_list (fst l1) (fst l2) (snd l1);
+  assert (fst l1 `ghost_map_disjoint` fst l2);
+  ghost_map_disjoint_mem_union' (fst l1) (fst l2) ();
+  assert (forall x . (ghost_map_mem x (fst l') \/ List.Tot.memP x (snd l')) <==> List.Tot.memP x l);
+  Classical.forall_intro (list_memP_map fst l);
+  Classical.forall_intro (list_memP_map fst (snd l1));
+  Classical.forall_intro (list_memP_map fst (snd l2));
+  assert (forall x . ~ (ghost_map_defined x (fst l') /\ List.Tot.memP x (List.Tot.map fst (snd l'))))
+
+#pop-options
 
 let map_group_concat (m1 m2: map_group) : map_group =
   FE.on_dom_g cbor_map #map_group_codom
@@ -745,6 +906,93 @@ let map_group_equiv_intro
 = Classical.forall_intro_2 (fun l l' -> Classical.move_requires (prf12 l) l');
   Classical.forall_intro_2 (fun l l' -> Classical.move_requires (prf21 l) l')
 
+let map_group_equiv_intro_equiv
+  (m1 m2: map_group)
+  (prf: (l: cbor_map) ->
+    (l': _) ->
+    Lemma
+    (FStar.GSet.mem l' (m1 l) <==> FStar.GSet.mem l' (m2 l))
+  )
+: Lemma
+  (map_group_equiv m1 m2)
+= map_group_equiv_intro m1 m2 (fun l l' -> prf l l') (fun l l' -> prf l l')
+
+let map_group_equiv_intro_equiv_rec
+  (m1 m2: map_group)
+  (prf: (l: cbor_map) ->
+    (prf: (
+      (l1: cbor_map { List.Tot.length l1 < List.Tot.length l }) -> Lemma
+      (m1 l1 == m2 l1)
+    )) ->
+    (l': _) ->
+    Lemma
+    (FStar.GSet.mem l' (m1 l) <==> FStar.GSet.mem l' (m2 l))
+  )
+: Lemma
+  (map_group_equiv m1 m2)
+= let rec prf' (l: cbor_map) (l': _) : Lemma
+    (ensures FStar.GSet.mem l' (m1 l) <==> FStar.GSet.mem l' (m2 l))
+    (decreases (List.Tot.length l))
+  = prf l (fun l1 ->
+      Classical.forall_intro (prf' l1);
+      prf' l1 l'; assert (m1 l1 `FStar.GSet.equal` m2 l1)
+    )
+    l'
+  in
+  map_group_equiv_intro_equiv m1 m2 prf'
+
+let map_group_equiv_intro_rec
+  (m1 m2: map_group)
+  (prf12: (l: cbor_map) ->
+    (prf: (
+      (l1: cbor_map { List.Tot.length l1 < List.Tot.length l }) -> Lemma
+      (m1 l1 == m2 l1)
+    )) ->
+    (l': _) ->
+    Lemma
+    (requires FStar.GSet.mem l' (m1 l))
+    (ensures FStar.GSet.mem l' (m2 l))
+  )
+  (prf21: (l: cbor_map) ->
+    (prf: (
+      (l1: cbor_map { List.Tot.length l1 < List.Tot.length l }) -> Lemma
+      (m1 l1 == m2 l1)
+    )) ->
+    (l': _) ->
+    Lemma
+    (requires FStar.GSet.mem l' (m2 l))
+    (ensures FStar.GSet.mem l' (m1 l))
+  )
+: Lemma
+  (map_group_equiv m1 m2)
+= map_group_equiv_intro_equiv_rec m1 m2 (fun l prf l' ->
+    Classical.move_requires (prf12 l prf) l';
+    Classical.move_requires (prf21 l prf) l'
+  )
+
+let ghost_map_disjoint_union_assoc_domain
+  (#key #value: Type)
+  (f1 f2 f3: ghost_map key value)
+: Lemma
+  (ensures (
+    (f1 `ghost_map_disjoint` f2 /\ (f1 `ghost_map_union` f2) `ghost_map_disjoint` f3) <==>
+      (f2 `ghost_map_disjoint` f3 /\ f1 `ghost_map_disjoint` (f2 `ghost_map_union` f3))
+  ))
+= ()
+
+let ghost_map_disjoint_union_assoc
+  (#key #value: Type)
+  (f1 f2 f3: ghost_map key value)
+: Lemma
+  (requires
+      (f1 `ghost_map_disjoint` f2 /\ (f1 `ghost_map_union` f2) `ghost_map_disjoint` f3) \/
+      (f2 `ghost_map_disjoint` f3 /\ f1 `ghost_map_disjoint` (f2 `ghost_map_union` f3))
+  )
+  (ensures
+    (f1 `ghost_map_union` (f2 `ghost_map_union` f3) == (f1 `ghost_map_union` f2) `ghost_map_union` f3)
+  )
+= assert ((f1 `ghost_map_union` (f2 `ghost_map_union` f3)) `FE.feq_g` ((f1 `ghost_map_union` f2) `ghost_map_union` f3))
+
 #push-options "--z3rlimit 16"
 
 #restart-solver
@@ -755,21 +1003,29 @@ let map_group_concat_assoc' (m1 m2 m3: map_group) : Lemma
     (map_group_concat (map_group_concat m1 m2) m3)
     (fun l l' -> 
       let (l1, l23) = map_group_concat_elim m1 (map_group_concat m2 m3) l l' in
+      ghost_map_disjoint_mem_union' (fst l1) (fst l23) ();
       let (l2, l3) = map_group_concat_elim m2 m3 (snd l1) l23 in
+      ghost_map_disjoint_mem_union' (fst l2) (fst l3) ();
       assert (FStar.GSet.mem l1 (m1 l));
       assert (FStar.GSet.mem l2 (m2 (snd l1)));
       assert (FStar.GSet.mem l3 (m3 (snd l2)));
-      let l12 = (fst l1 `List.Tot.append` fst l2, snd l2) in
+      let l12 = (fst l1 `ghost_map_union` fst l2, snd l2) in
+      ghost_map_disjoint_mem_union' (fst l1) (fst l2) ();
       assert (map_group_concat_witness_pred m1 m2 l l12 (l1, l2));
-      List.Tot.append_assoc (fst l1) (fst l2) (fst l3);
+      ghost_map_disjoint_union_assoc (fst l1) (fst l2) (fst l3);
+      ghost_map_disjoint_mem_union' (fst l12) (fst l3) ();
       assert (map_group_concat_witness_pred (map_group_concat m1 m2) m3 l l' (l12, l3))
     )
-    (fun l l' -> 
+    (fun l l' ->
       let (l12, l3) = map_group_concat_elim (map_group_concat m1 m2) m3 l l' in
+      ghost_map_disjoint_mem_union' (fst l12) (fst l3) ();
       let (l1, l2) = map_group_concat_elim m1 m2 l l12 in
-      let l23 = (fst l2 `List.Tot.append` fst l3, snd l3) in
+      ghost_map_disjoint_mem_union' (fst l1) (fst l2) ();
+      let l23 = (fst l2 `ghost_map_union` fst l3, snd l3) in
+      ghost_map_disjoint_mem_union' (fst l2) (fst l3) ();
       assert (map_group_concat_witness_pred m2 m3 (snd l1) l23 (l2, l3));
-      List.Tot.append_assoc (fst l1) (fst l2) (fst l3);
+      ghost_map_disjoint_union_assoc (fst l1) (fst l2) (fst l3);
+      ghost_map_disjoint_mem_union' (fst l1) (fst l23) ();
       assert (map_group_concat_witness_pred m1 (map_group_concat m2 m3) l l' (l1, l23))
     )
 
@@ -781,17 +1037,9 @@ let map_group_concat_assoc m1 m2 m3 =
 let map_group_mk_cut (cut: typ) : map_group =
   FE.on_dom_g cbor_map #map_group_codom (fun l -> 
     if List.Tot.for_all (notp (FStar.Ghost.Pull.pull (matches_map_group_entry cut any))) l
-    then FStar.GSet.singleton ([], l)
-    else FStar.GSet.empty
+    then map_group_nop l
+    else map_group_always_false l
   )
-
-let list_append_l_nil
-  (#t: Type)
-  (l: list t)
-: Lemma
-  (l `List.Tot.append` [] == l)
-  [SMTPat (l `List.Tot.append` [])]
-= List.Tot.append_l_nil l
 
 #restart-solver
 let map_group_concat_nop_l
@@ -801,9 +1049,12 @@ let map_group_concat_nop_l
 = map_group_equiv_intro
     (map_group_concat map_group_nop m)
     m
-    (fun l l' -> ())
-    (fun l l' -> 
-      assert (map_group_concat_witness_pred map_group_nop m l l' (([], l), l'))
+    (fun l l' ->
+      let (l1, l2) = map_group_concat_elim map_group_nop m l l' in
+      assert (fst l' `ghost_map_feq` fst l2)
+    )
+    (fun l l' ->
+      assert (map_group_concat_witness_pred map_group_nop m l l' ((ghost_map_empty, l), l'))
     )
 
 let map_group_concat_nop_r
@@ -813,9 +1064,12 @@ let map_group_concat_nop_r
 = map_group_equiv_intro
     (map_group_concat m map_group_nop)
     m
-    (fun l l' -> ())
+    (fun l l' ->
+      let (l1, l2) = map_group_concat_elim m map_group_nop l l' in
+      assert (fst l' `ghost_map_feq` fst l1)
+    )
     (fun l l' -> 
-      assert (map_group_concat_witness_pred m map_group_nop l l' (l', ([], snd l')))
+      assert (map_group_concat_witness_pred m map_group_nop l l' (l', (ghost_map_empty, snd l')))
     )
 
 #restart-solver
@@ -824,12 +1078,11 @@ let map_group_cut_eq
   (m: map_group)
 : Lemma
   (map_group_cut cut m == (map_group_mk_cut cut `map_group_concat` m))
-= map_group_equiv_intro
+= map_group_concat_nop_l m;
+  map_group_equiv_intro
     (map_group_cut cut m)
     (map_group_mk_cut cut `map_group_concat` m)
-    (fun l l' ->
-       assert (map_group_concat_witness_pred (map_group_mk_cut cut) m l l' (([], l), l'))
-    )
+    (fun l l' -> ())
     (fun l l' -> ())
 
 let bound_map_group
@@ -841,7 +1094,7 @@ let bound_map_group
   )
 : map_group
 = FE.on_dom_g cbor_map #map_group_codom
-    (fun l -> if List.Tot.length l >= List.Tot.length l0 then FStar.GSet.singleton ([], l) else m l)
+    (fun l -> if List.Tot.length l >= List.Tot.length l0 then map_group_nop l else m l)
 
 let bound_map_group_ext
   (l0: list (Cbor.raw_data_item & Cbor.raw_data_item))
@@ -869,7 +1122,7 @@ let rec map_group_zero_or_more'
   (decreases (List.Tot.length l))
 = let res1 = m l in
   if FStar.StrongExcludedMiddle.strong_excluded_middle (res1 == FStar.GSet.empty)
-  then FStar.GSet.singleton ([], l)
+  then map_group_nop l
   else map_group_concat m (bound_map_group l (map_group_zero_or_more' m)) l
 
 let map_group_zero_or_more m =
@@ -881,28 +1134,17 @@ let map_group_zero_or_more_eq
 : Lemma
   (ensures (map_group_zero_or_more m l == (let res1 = m l in
     if FStar.StrongExcludedMiddle.strong_excluded_middle (res1 == FStar.GSet.empty)
-    then FStar.GSet.singleton ([], l)
+    then map_group_nop l
     else map_group_concat m (bound_map_group l (map_group_zero_or_more m)) l
   )))
   (decreases (List.Tot.length l))
 = assert (forall l . map_group_zero_or_more m l == map_group_zero_or_more' m l);
   assert_norm (map_group_zero_or_more' m l == (let res1 = m l in
     if FStar.StrongExcludedMiddle.strong_excluded_middle (res1 == FStar.GSet.empty)
-    then FStar.GSet.singleton ([], l)
+    then map_group_nop l
     else map_group_concat m (bound_map_group l (map_group_zero_or_more' m)) l
   ));
   bound_map_group_ext l (map_group_zero_or_more m) (map_group_zero_or_more' m)
-
-let rec list_ghost_assoc_memP
-  (#key #value: Type)
-  (k: key)
-  (l: list (key & value))
-: Lemma
-  (ensures (Some? (Cbor.list_ghost_assoc k l) <==> List.Tot.memP k (List.Tot.map fst l)))
-  (decreases l)
-= match l with
-  | [] -> ()
-  | _ :: q -> list_ghost_assoc_memP k q
 
 let rec list_filter_and_extract_matches_map_group_entry_literal_memP_intro
   (k: Cbor.raw_data_item)
@@ -967,7 +1209,7 @@ let map_group_match_item_for_eq
   (ensures (
     map_group_match_item_for k ty l `FStar.GSet.equal` begin match list_filter_and_extract (FStar.Ghost.Pull.pull (matches_map_group_entry (t_literal k) ty)) l with
     | None -> FStar.GSet.empty
-    | Some (ll, kv, lr) -> FStar.GSet.singleton ([kv], ll `List.Tot.append` lr)
+    | Some (ll, kv, lr) -> FStar.GSet.singleton (ghost_map_singleton (fst kv) (snd kv), ll `List.Tot.append` lr)
     end
   ))
 = map_group_match_item_alt_correct (t_literal k) ty l;
@@ -1021,100 +1263,192 @@ let rec list_filter_append
   | [] -> ()
   | _ :: q -> list_filter_append f q l2
 
-let gset_collect_bound_map_group_length_lt
-  (l: cbor_map)
-  (m: map_group)
-  (s: FStar.GSet.set cbor_map)
-: Lemma
-  (requires (forall (x: cbor_map) . FStar.GSet.mem x s ==> List.Tot.length x < List.Tot.length l))
-  (ensures (
-    gset_collect (bound_map_group l m) s `FStar.GSet.equal` gset_collect m s
-  ))
-= ()
-
 let map_group_match_item_length
   (key value: typ)
   (l: cbor_map)
-  (l': list (Cbor.raw_data_item & Cbor.raw_data_item))
+  l'
 : Lemma
   (requires FStar.GSet.mem l' (map_group_match_item key value l))
-  (ensures List.Tot.length l' < List.Tot.length l)
+  (ensures List.Tot.length (snd l') < List.Tot.length l)
   [SMTPat (FStar.GSet.mem l' (map_group_match_item key value l))]
 = let (l1, kv, l2) = FStar.IndefiniteDescription.indefinite_description_ghost _ (map_group_match_item_witness_pred key value l l') in
   List.Tot.append_length l1 (kv :: l2);
   List.Tot.append_length l1 l2
 
-#push-options "--z3rlimit 16"
+let ghost_map_filter
+  (#key #value: Type)
+  (f: (key & value) -> GTot bool)
+  (m: ghost_map key value)
+: ghost_map key value
+= FE.on_dom_g _ (fun k ->
+    match m k with
+    | Some v -> if f (k, v) then Some v else None
+    | None -> None
+  )
 
-#restart-solver
-let rec map_group_zero_or_more_match_item_eq
-  (key value: typ)
+let ghost_map_filter_ext
+  (#key #value: Type)
+  (f1 f2: (key & value) -> GTot bool)
+  (m: ghost_map key value)
+: Lemma
+  (requires forall x . f1 x == f2 x)
+  (ensures ghost_map_filter f1 m == ghost_map_filter f2 m)
+= ghost_map_equiv (ghost_map_filter f1 m) (ghost_map_filter f2 m)
+
+let ghost_map_of_list
+  (#key #value: Type)
+  (l: list (key & value))
+: ghost_map key value
+= FE.on_dom_g _ (fun k -> Cbor.list_ghost_assoc k l)
+
+let ghost_map_of_list_singleton
+  (#key #value: Type)
+  (kv: (key & value))
+: Lemma
+  (ghost_map_of_list [kv] == ghost_map_singleton (fst kv) (snd kv))
+  [SMTPat (ghost_map_of_list [kv])]
+= assert (ghost_map_of_list [kv] `ghost_map_feq` ghost_map_singleton (fst kv) (snd kv))
+
+let ghost_map_of_list_singleton'
+  (#key #value: Type)
+  (k: key)
+  (v: value)
+: Lemma
+  (ghost_map_of_list [k, v] == ghost_map_singleton k v)
+  [SMTPat (ghost_map_singleton k v)]
+= ghost_map_of_list_singleton (k, v)
+
+let rec list_ghost_assoc_append
+  (#key #value: Type)
+  (l1 l2: list (key & value))
+  (x: key)
+: Lemma
+  (ensures (Cbor.list_ghost_assoc x (l1 `List.Tot.append` l2) == begin match Cbor.list_ghost_assoc x l1 with
+  | Some v -> Some v
+  | None -> Cbor.list_ghost_assoc x l2
+  end))
+  (decreases l1)
+= match l1 with
+  | [] -> ()
+  | _ :: q -> list_ghost_assoc_append q l2 x
+
+let ghost_map_of_list_append
+  (#key #value: Type)
+  (l1 l2: list (key & value))
+: Lemma
+  (ghost_map_of_list (List.Tot.append l1 l2) == ghost_map_of_list l1 `ghost_map_union` ghost_map_of_list l2)
+= Classical.forall_intro (list_ghost_assoc_append l1 l2);
+  assert
+    (ghost_map_of_list (List.Tot.append l1 l2) `ghost_map_feq`
+      (ghost_map_of_list l1 `ghost_map_union` ghost_map_of_list l2))
+
+let ghost_map_of_list_mem_gen
+  (#key #value: Type)
+  (l: list (key & value))
+  (prf: squash (List.Tot.no_repeats_p (List.Tot.map fst l)))
+  (x: (key & value))
+: Lemma
+  (ghost_map_mem x (ghost_map_of_list l) <==> List.Tot.memP x l)
+= list_ghost_assoc_memP_strong (fst x) (snd x) l
+
+let ghost_map_of_list_mem
+  (l: cbor_map)
+  (x: (Cbor.raw_data_item & Cbor.raw_data_item))
+: Lemma
+  (ghost_map_mem x (ghost_map_of_list l) <==> List.Tot.memP x l)
+= ghost_map_of_list_mem_gen l () x
+
+let list_filter_memP
+  (#t: Type)
+  (f: t -> bool)
+  (l: list t)
+  (x: t)
+: Lemma
+  (List.Tot.memP x (List.Tot.filter f l) <==> (List.Tot.memP x l /\ f x))
+= ()
+
+let ghost_map_filter_of_list
+  (f: _ -> bool)
   (l: cbor_map)
 : Lemma
-  (ensures map_group_zero_or_more (map_group_match_item key value) l `FStar.GSet.equal`
-    FStar.GSet.singleton (List.Tot.filter (notp (FStar.Ghost.Pull.pull (matches_map_group_entry key value))) l))
-  (decreases (List.Tot.length l))
-=
-  let m = map_group_match_item key value in
-  let f = FStar.Ghost.Pull.pull (matches_map_group_entry key value) in
-  let gset_collect_map_group_zero_or_more_match_item_eq
-    (s: FStar.GSet.set cbor_map)
-  : Lemma
-    (requires (forall (x: cbor_map) . FStar.GSet.mem x s ==> List.Tot.length x < List.Tot.length l))
-    (ensures gset_collect (map_group_zero_or_more m) s `FStar.GSet.equal`
-      gset_map (List.Tot.filter (notp f)) s
+  (ghost_map_filter f (ghost_map_of_list l) == ghost_map_of_list (List.Tot.filter f l))
+= ghost_map_equiv_intro'
+    (ghost_map_filter f (ghost_map_of_list l))
+    (ghost_map_of_list (List.Tot.filter f l))
+    (fun (k, v) -> 
+      list_ghost_assoc_memP_strong k v l;
+      list_filter_memP f l (k, v);
+      list_ghost_assoc_memP_strong k v (List.Tot.filter f l)
     )
-  = gset_equal_intro
-      (gset_collect (map_group_zero_or_more m) s)
-      (gset_map (List.Tot.filter (notp f)) s)
-      (fun l' ->
-        let l1 = FStar.IndefiniteDescription.indefinite_description_ghost _ (gset_collect_witness_pred (map_group_zero_or_more m) s l') in
-        map_group_zero_or_more_match_item_eq key value l1;
-        assert (gset_map_witness_pred (List.Tot.filter (notp f)) s l' l1)
-      )
-      (fun l' ->
-        let l1 = FStar.IndefiniteDescription.indefinite_description_ghost _ (gset_map_witness_pred (List.Tot.filter (notp f)) s l') in
-        map_group_zero_or_more_match_item_eq key value l1;
-        assert (gset_collect_witness_pred (map_group_zero_or_more m) s l' l1)
-      )
-  in
-  map_group_zero_or_more_eq m l;
-  let res1 = apply_map_group m l in
-  map_group_match_item_alt_correct key value l;
-  match list_filter_and_extract f l with
-  | None ->
-    assert (apply_map_group m l `FStar.GSet.equal` FStar.GSet.empty);
-    list_for_all_implies_filter (notp f) l
-  | Some (l1, kv, l2) ->
-    assert (~ (apply_map_group m l == FStar.GSet.empty));
-    gset_collect_bound_map_group_length_lt l (map_group_zero_or_more m) res1;
-    gset_collect_map_group_zero_or_more_match_item_eq res1;
-    assert (map_group_zero_or_more m l == gset_map (List.Tot.filter (notp f)) res1);
-    gset_equal_intro
-      (FStar.GSet.singleton (List.Tot.filter (notp f) l)) 
-      (gset_map (List.Tot.filter (notp f)) res1)
-      (fun l' ->
-        assert (l' == List.Tot.filter (notp f) l);
-        assert (FStar.GSet.mem (l1 `List.Tot.append` l2) res1);
-        list_filter_append (notp f) l1 l2;
-        list_filter_append (notp f) l1 (kv :: l2);
-        assert (gset_map_witness_pred (List.Tot.filter (notp f)) res1 l' (l1 `List.Tot.append` l2))
-      )
-      (fun l' ->
-        let l1 = FStar.IndefiniteDescription.indefinite_description_ghost _ (gset_map_witness_pred (List.Tot.filter (notp f)) res1 l') in
-        assert (FStar.GSet.mem l1 res1);
-        let (ll, kv, lr) = map_group_match_item_elim key value l l1 in
-        list_filter_append (notp f) ll lr;
-        list_filter_append (notp f) ll (kv :: lr);
-        assert (l == ll `List.Tot.append` (kv :: lr));
-        assert (l1 == ll `List.Tot.append` lr);
-        assert (f kv);
-        assert (l' == List.Tot.filter (notp f) l1);
-        assert (List.Tot.filter (notp f) (kv :: lr) == List.Tot.filter (notp f) lr);
-        assert (l' == List.Tot.filter (notp f) l)
-      )
 
-#pop-options
+let rec list_for_all_not_implies_filter
+  (#key #value: Type)
+  (f: (key & value) -> GTot bool)
+  (l: list (key & value))
+: Lemma
+  (requires (List.Tot.for_all (notp (FStar.Ghost.Pull.pull f)) l))
+  (ensures (ghost_map_filter f (ghost_map_of_list l) `ghost_map_feq` ghost_map_empty))
+= match l with
+  | [] -> ()
+  | _ :: q -> list_for_all_not_implies_filter f q
+
+#restart-solver
+let gset_is_empty
+  (#t: Type)
+  (s: FStar.GSet.set t)
+: Ghost (option t)
+    (requires True)
+    (ensures fun res -> 
+    (None? res <==> s == FStar.GSet.empty) /\
+    begin match res with
+    | None -> True
+    | Some x -> FStar.GSet.mem x s
+    end
+    )
+= if FStar.StrongExcludedMiddle.strong_excluded_middle (exists x . FStar.GSet.mem x s)
+  then Some (FStar.IndefiniteDescription.indefinite_description_ghost _ (fun x -> FStar.GSet.mem x s))
+  else begin
+    assert (s `FStar.GSet.equal` FStar.GSet.empty);
+    None
+  end
+
+#restart-solver
+let map_group_zero_or_more_zero_or_one_eq
+  (m: map_group)
+: Lemma
+  (map_group_zero_or_more (map_group_zero_or_one m) == map_group_zero_or_more m)
+=
+  assert ((ghost_map_empty #Cbor.raw_data_item #Cbor.raw_data_item  `ghost_map_union` ghost_map_empty) `ghost_map_feq` ghost_map_empty);
+  map_group_equiv_intro_rec
+    (map_group_zero_or_more (map_group_zero_or_one m))
+    (map_group_zero_or_more m)
+    (fun l prf l' ->
+      map_group_zero_or_more_eq (map_group_zero_or_one m) l;
+      map_group_zero_or_more_eq m l;
+      assert (~ (map_group_zero_or_one m l == FStar.GSet.empty));
+      Classical.forall_intro prf;
+      bound_map_group_ext l (map_group_zero_or_more (map_group_zero_or_one m)) (map_group_zero_or_more m);
+      let (l1, l2) = map_group_concat_elim (map_group_zero_or_one m) (bound_map_group l (map_group_zero_or_more m)) l l' in
+      ()
+    )
+    (fun l prf l' ->
+      map_group_zero_or_more_eq (map_group_zero_or_one m) l;
+      map_group_zero_or_more_eq m l;
+      assert (~ (map_group_zero_or_one m l == FStar.GSet.empty));
+      Classical.forall_intro prf;
+      bound_map_group_ext l (map_group_zero_or_more (map_group_zero_or_one m)) (map_group_zero_or_more m);
+      match gset_is_empty (m l) with
+      | None ->
+        assert (map_group_concat_witness_pred (map_group_zero_or_one m) (bound_map_group l (map_group_zero_or_more m)) l l'
+          (
+            (ghost_map_empty, l),
+            (ghost_map_empty, l)
+          )
+        )
+      | _ -> 
+        let (l1, l2) = map_group_concat_elim m (bound_map_group l (map_group_zero_or_more m)) l l' in
+        ()
+    )
 
 let apply_map_group_det (m: map_group) (l: cbor_map) : Pure map_group_result
   (requires True)
@@ -1123,13 +1457,21 @@ let apply_map_group_det (m: map_group) (l: cbor_map) : Pure map_group_result
   if FStar.StrongExcludedMiddle.strong_excluded_middle (s == FStar.GSet.empty)
   then MapGroupFail
   else if FStar.StrongExcludedMiddle.strong_excluded_middle (exists x . s == FStar.GSet.singleton x)
-  then MapGroupDet (FStar.IndefiniteDescription.indefinite_description_ghost _ (fun x -> s == FStar.GSet.singleton x))
+  then MapGroupDet (snd (FStar.IndefiniteDescription.indefinite_description_ghost _ (fun x -> s == FStar.GSet.singleton x)))
   else MapGroupNonDet
 
-let apply_map_group_det_eq_singleton (m: map_group) (l: cbor_map) x : Lemma
+#restart-solver
+let apply_map_group_det_eq_singleton (m: map_group) (l: cbor_map) (x : (_ & list _)) : Lemma
   (requires (m l `FStar.GSet.equal` FStar.GSet.singleton x))
-  (ensures (apply_map_group_det m l == MapGroupDet x))
-= ()
+  (ensures (apply_map_group_det m l == MapGroupDet (snd x)))
+= let s = m l in
+  assert (s == FStar.GSet.singleton x);
+  if FStar.StrongExcludedMiddle.strong_excluded_middle (s == FStar.GSet.empty)
+  then assert (x `FStar.GSet.mem` FStar.GSet.empty)
+  else begin
+    assert (exists x . s == FStar.GSet.singleton x);
+    assert (MapGroupDet? (apply_map_group_det m l))
+  end
 
 let apply_map_group_det_always_false (l: cbor_map) : Lemma
   (apply_map_group_det map_group_always_false l == MapGroupFail)
@@ -1149,24 +1491,21 @@ let apply_map_group_det_map_group_equiv (m1 m2: map_group) : Lemma
     (forall l . apply_map_group_det m1 l == apply_map_group_det m2 l)
   )
   (ensures m1 == m2)
-= assert (m1 `map_group_equiv` m2)
-
-let gset_collect_empty
-  (m: map_group)
-  (l: FStar.GSet.set cbor_map)
-: Lemma
-  (requires l `FStar.GSet.equal` FStar.GSet.empty)
-  (ensures gset_collect m l `FStar.GSet.equal` FStar.GSet.empty)
-= ()
-
-let gset_collect_singleton
-  (m: map_group)
-  (l: FStar.GSet.set cbor_map)
-  (x: cbor_map)
-: Lemma
-  (requires l `FStar.GSet.equal` FStar.GSet.singleton x)
-  (ensures gset_collect m l `FStar.GSet.equal` m x)
-= ()
+= map_group_equiv_intro m1 m2
+    (fun l l' ->
+      let MapGroupDet s1 = apply_map_group_det m1 l in
+      let (k1, l1) = FStar.IndefiniteDescription.indefinite_description_ghost _ (fun s1 -> m1 l == FStar.GSet.singleton s1) in
+      let (k2, l2) = FStar.IndefiniteDescription.indefinite_description_ghost _ (fun s2 -> m2 l == FStar.GSet.singleton s2) in
+      assert (l1 == l2);
+      ghost_map_equiv k1 k2
+    )
+    (fun l l' ->
+      let MapGroupDet s1 = apply_map_group_det m1 l in
+      let (k1, l1) = FStar.IndefiniteDescription.indefinite_description_ghost _ (fun s1 -> m1 l == FStar.GSet.singleton s1) in
+      let (k2, l2) = FStar.IndefiniteDescription.indefinite_description_ghost _ (fun s2 -> m2 l == FStar.GSet.singleton s2) in
+      assert (l1 == l2);
+      ghost_map_equiv k1 k2
+    )
 
 let apply_map_group_det_choice (m1 m2: map_group) (l: cbor_map) : Lemma
   (match apply_map_group_det m1 l with
@@ -1176,17 +1515,66 @@ let apply_map_group_det_choice (m1 m2: map_group) (l: cbor_map) : Lemma
   )
 = ()
 
+#push-options "--z3rlimit 16"
+
+#restart-solver
 let apply_map_group_det_concat (m1 m2: map_group) (l: cbor_map) : Lemma
   (match apply_map_group_det m1 l with
   | MapGroupFail -> apply_map_group_det (m1 `map_group_concat` m2) l == MapGroupFail
   | MapGroupDet l1 -> apply_map_group_det (m1 `map_group_concat` m2) l == apply_map_group_det m2 l1
   | _ -> True)
 = match apply_map_group_det m1 l with
-  | MapGroupFail -> 
-    gset_collect_empty m2 (apply_map_group m1 l)
-  | MapGroupDet l1 ->
-    gset_collect_singleton m2 (apply_map_group m1 l) l1
+  | MapGroupFail ->
+    assert (map_group_concat m1 m2 l `FStar.GSet.equal` FStar.GSet.empty)
+  | MapGroupDet lr1 ->
+    let l1 = FStar.IndefiniteDescription.indefinite_description_ghost _ (fun x -> m1 l == FStar.GSet.singleton x) in
+    begin match apply_map_group_det m2 lr1 with
+    | MapGroupFail -> assert (map_group_concat m1 m2 l `FStar.GSet.equal` FStar.GSet.empty)
+    | MapGroupDet lr2 ->
+      let l2 = FStar.IndefiniteDescription.indefinite_description_ghost _ (fun x -> m2 lr1 == FStar.GSet.singleton x) in
+      let l0 = (ghost_map_union (fst l1) (fst l2), snd l2) in
+      gset_equal_intro
+        (map_group_concat m1 m2 l)
+        (FStar.GSet.singleton l0)
+        (fun _ -> ())
+        (fun _ ->
+          assert (map_group_concat_witness_pred m1 m2 l l0
+            (l1, l2)
+          )
+        )
+    | MapGroupNonDet ->
+      let Some l2 = gset_is_empty (m2 lr1) in
+      let l0 = (ghost_map_union (fst l1) (fst l2), snd l2) in
+      assert (map_group_concat_witness_pred m1 m2 l l0
+        (l1, l2)
+      );
+      assert (FStar.GSet.mem l0 (map_group_concat m1 m2 l));
+      assert (~ (map_group_concat m1 m2 l == FStar.GSet.empty));
+      if FStar.StrongExcludedMiddle.strong_excluded_middle (exists x . map_group_concat m1 m2 l == FStar.GSet.singleton x)
+      then begin
+        assert (map_group_concat m1 m2 l `FStar.GSet.equal` FStar.GSet.singleton l0);
+        gset_equal_intro
+          (m2 lr1)
+          (FStar.GSet.singleton l2)
+          (fun l2' ->
+            let l0' = (ghost_map_union (fst l1) (fst l2'), snd l2') in
+            assert (map_group_concat_witness_pred m1 m2 l l0'
+              (l1, l2')
+            );
+            assert (FStar.GSet.mem l0' (map_group_concat m1 m2 l));
+            assert (l0' == l0);
+            ghost_map_disjoint_mem_union' (fst l1) (fst l2') ();
+            ghost_map_disjoint_mem_union' (fst l1) (fst l2) ();
+            ghost_map_equiv (fst l2') (fst l2);
+            assert (l2' == l2)
+          )
+          (fun _ -> ())
+      end
+      else ()
+    end
   | _ -> ()
+
+#pop-options
 
 let apply_map_group_det_mk_cut cut l = ()
 
@@ -1216,7 +1604,220 @@ let apply_map_group_det_match_item_for
     list_for_all_implies_filter (notp (FStar.Ghost.Pull.pull (matches_map_group_entry (t_literal k) ty))) lr;
     list_filter_append (notp (FStar.Ghost.Pull.pull (matches_map_group_entry (t_literal k) ty))) ll (kv :: lr);
     apply_map_group_det_eq_singleton (map_group_match_item_for k ty) l
-      (List.Tot.filter (notp (FStar.Ghost.Pull.pull (matches_map_group_entry (t_literal k) ty))) l)
+      (ghost_map_singleton (fst kv) (snd kv),
+        List.Tot.filter (notp (FStar.Ghost.Pull.pull (matches_map_group_entry (t_literal k) ty))) l)
+
+// FIXME: swap `notp f` with `f`?
+let map_group_filter_item
+  (f: (Cbor.raw_data_item & Cbor.raw_data_item) -> bool)
+  (l: cbor_map)
+: GTot (ghost_map Cbor.raw_data_item Cbor.raw_data_item & list (Cbor.raw_data_item & Cbor.raw_data_item))
+=
+  ghost_map_filter (notp f) (ghost_map_of_list l),
+    List.Tot.filter f l
+
+let map_group_item_post_filter
+  (f: (Cbor.raw_data_item & Cbor.raw_data_item) -> bool)
+  (l: cbor_map)
+: Lemma
+  (map_group_item_post l (map_group_filter_item f l))
+  [SMTPat (map_group_filter_item f l)]
+= let l' = map_group_filter_item f l in
+  assert (snd l' `is_sublist_of` l);
+  ghost_map_filter_of_list (notp f) l;
+  list_ghost_assoc_memP_strong' l ();
+  assert (forall x . (ghost_map_mem x (fst l') \/ List.Tot.memP x (snd l')) <==> List.Tot.memP x l);
+  Classical.forall_intro (list_memP_map fst l);
+  Classical.forall_intro (list_memP_map fst (snd l'));
+  assert (forall x . ~ (ghost_map_defined x (fst l') /\ List.Tot.memP x (List.Tot.map fst (snd l'))))
+
+let map_group_filter
+  f
+= FE.on_dom_g cbor_map #map_group_codom (fun l ->
+    FStar.GSet.singleton (map_group_filter_item f l)
+  )
+
+let apply_map_group_det_filter
+  f l
+= apply_map_group_det_eq_singleton (map_group_filter f) l (map_group_filter_item f l)
+
+let list_filter_implies_2' (#t: Type) (p1 p2: t -> bool) : Lemma
+  (requires (forall (x: t) . p1 x ==> p2 x))
+  (ensures forall  (l: list t) . List.Tot.filter p1 (List.Tot.filter p2 l) == List.Tot.filter p1 l)
+= Classical.forall_intro (fun l -> Classical.move_requires (list_filter_implies_2 p1 p2) l)
+
+let list_memP_equiv_map_no_repeats
+  (#key #value: Type)
+  (l1 l2: list (key & value))
+: Lemma
+  (requires (
+    List.Tot.no_repeats_p (List.Tot.map fst l1) /\
+    (forall x . List.Tot.memP x l1 <==> List.Tot.memP x l2) /\
+    List.Tot.length l1 >= List.Tot.length l2
+  ))
+  (ensures (
+    List.Tot.length l1 == List.Tot.length l2 /\
+    List.Tot.no_repeats_p (List.Tot.map fst l2)
+  ))
+= Classical.forall_intro (list_memP_map fst l1);
+  Classical.forall_intro (list_memP_map fst l2);
+  list_memP_equiv_no_repeats (List.Tot.map fst l1) (List.Tot.map fst l2)
+
+let ghost_map_of_list_ext
+  (#key #value: Type)
+  (l1 l2: list (key & value))
+: Lemma
+  (requires (
+    List.Tot.no_repeats_p (List.Tot.map fst l1) /\
+    (forall x . List.Tot.memP x l1 <==> List.Tot.memP x l2) /\
+    List.Tot.length l1 >= List.Tot.length l2
+  ))
+  (ensures (
+    List.Tot.length l1 == List.Tot.length l2 /\
+    List.Tot.no_repeats_p (List.Tot.map fst l2) /\
+    ghost_map_of_list l1 == ghost_map_of_list l2
+  ))
+= list_memP_equiv_map_no_repeats l1 l2;
+  Classical.forall_intro (ghost_map_of_list_mem_gen l1 ());
+  Classical.forall_intro (ghost_map_of_list_mem_gen l2 ());
+  ghost_map_equiv (ghost_map_of_list l1) (ghost_map_of_list l2)
+
+#restart-solver
+let map_group_zero_or_one_match_item_filter_matched
+  (key value: typ)
+  (p: (Cbor.raw_data_item & Cbor.raw_data_item) -> bool)
+  (l: cbor_map)
+  ll kv lr
+: Lemma
+  (requires (
+    (forall x . p x ==> notp (FStar.Ghost.Pull.pull (matches_map_group_entry key value)) x) /\
+    l == ll `List.Tot.append` (kv :: lr) /\
+    matches_map_group_entry key value kv
+  ))
+  (ensures (
+    ghost_map_singleton (fst kv) (snd kv) `ghost_map_union` ghost_map_filter (notp p) (ghost_map_of_list (ll `List.Tot.append` lr)) ==
+      ghost_map_filter (notp p) (ghost_map_of_list l)
+  ))
+= List.Tot.append_length ll (kv :: lr);
+  List.Tot.append_length ll lr;
+  Classical.forall_intro (List.Tot.append_memP ll (kv :: lr));
+  Classical.forall_intro (List.Tot.append_memP ll lr);
+  ghost_map_of_list_ext (ll `List.Tot.append` (kv :: lr)) (kv :: ll `List.Tot.append` lr);
+  ghost_map_filter_of_list (notp p) l;
+  ghost_map_filter_of_list (notp p) (kv :: ll `List.Tot.append` lr);
+  list_filter_append (notp p) [kv] (ll `List.Tot.append` lr);
+  ghost_map_of_list_append (List.Tot.filter (notp p) [kv]) (List.Tot.filter (notp p) (ll `List.Tot.append` lr));
+  ghost_map_filter_of_list (notp p) (ll `List.Tot.append` lr)
+
+#restart-solver
+let map_group_zero_or_one_match_item_filter
+  key value p
+= map_group_equiv_intro
+    (map_group_zero_or_one (map_group_match_item key value) `map_group_concat` map_group_filter p)
+    (map_group_filter p)
+    (fun l l' ->
+      match gset_is_empty (map_group_match_item key value l) with
+      | None -> map_group_concat_nop_l (map_group_filter p)
+      | Some _ ->
+        let (l1, _) = map_group_concat_elim (map_group_zero_or_one (map_group_match_item key value)) (map_group_filter p) l l' in
+        let (ll, kv, lr) = map_group_match_item_elim key value l l1 in
+        list_filter_append p ll (kv :: lr);
+        list_filter_append p ll lr;
+        assert (fst l1 == ghost_map_singleton (fst kv) (snd kv));
+        assert (map_group_filter p (snd l1) == FStar.GSet.singleton (map_group_filter_item p (snd l1)));
+        map_group_zero_or_one_match_item_filter_matched key value p l ll kv lr
+    )
+    (fun l l' ->
+      match gset_is_empty (map_group_match_item key value l) with
+      | None -> map_group_concat_nop_l (map_group_filter p)
+      | Some l1 ->
+        let (ll, kv, lr) = map_group_match_item_elim key value l l1 in
+        list_filter_append p ll (kv :: lr);
+        list_filter_append p ll lr;
+        assert (snd l' == List.Tot.filter p (snd l1));
+        map_group_zero_or_one_match_item_filter_matched key value p l ll kv lr;
+        assert (map_group_concat_witness_pred (map_group_zero_or_one (map_group_match_item key value)) (map_group_filter p) l l' (l1, (ghost_map_filter (notp p) (ghost_map_of_list (ll `List.Tot.append` lr)), List.Tot.filter p (snd l1))))
+    )
+
+#push-options "--z3rlimit 32"
+
+#restart-solver
+let map_group_concat_bound_map_group_elim
+  (m1 m2: map_group)
+  (l1 l2: cbor_map)
+  (prf: (l': _) -> Lemma
+    (requires (FStar.GSet.mem l' (m1 l1)))
+    (ensures (List.Tot.length (snd l') < List.Tot.length l2))
+  )
+: Lemma
+  ((m1 `map_group_concat` bound_map_group l2 m2) l1 ==
+    (m1 `map_group_concat` m2) l1)
+= Classical.forall_intro (Classical.move_requires prf);
+  assert ((m1 `map_group_concat` bound_map_group l2 m2) l1 `FStar.GSet.equal`
+    (m1 `map_group_concat` m2) l1
+  )
+
+#pop-options
+
+#restart-solver
+let map_group_zero_or_one_bound_match_item_filter
+  (key value: typ)
+  (l: cbor_map)
+: Lemma
+  (ensures (
+    let p = notp (FStar.Ghost.Pull.pull (matches_map_group_entry key value)) in
+    (map_group_zero_or_one (map_group_match_item key value) `map_group_concat` bound_map_group l (map_group_filter p)) l == map_group_filter p l
+  ))
+= let p = notp (FStar.Ghost.Pull.pull (matches_map_group_entry key value)) in
+  map_group_match_item_alt_correct key value l;
+  match list_filter_and_extract (FStar.Ghost.Pull.pull (matches_map_group_entry key value)) l with
+  | None ->
+    assert (map_group_match_item key value l == FStar.GSet.empty);
+    assert ((ghost_map_empty #Cbor.raw_data_item #Cbor.raw_data_item `ghost_map_union` ghost_map_empty) `ghost_map_feq` ghost_map_empty);
+    list_for_all_implies_filter (notp (FStar.Ghost.Pull.pull (matches_map_group_entry key value))) l;
+    List.Tot.for_all_mem (notp (FStar.Ghost.Pull.pull (matches_map_group_entry key value))) l;
+    ghost_map_filter_of_list (notp p) l;
+    Classical.forall_intro (ghost_map_of_list_mem (List.Tot.filter p l));
+    Classical.forall_intro (list_filter_memP p l);
+    ghost_map_equiv (ghost_map_filter (notp p) (ghost_map_of_list l)) ghost_map_empty;
+    assert (map_group_filter p l `FStar.GSet.equal` FStar.GSet.singleton (ghost_map_empty, l));
+    assert (
+      ((map_group_zero_or_one (map_group_match_item key value) `map_group_concat` bound_map_group l (map_group_filter p)) l) `FStar.GSet.equal`
+      ((map_group_nop `map_group_concat` bound_map_group l (map_group_filter p)) l)
+    );
+    map_group_concat_nop_l (bound_map_group l (map_group_filter p));
+    assert (bound_map_group l (map_group_filter p) l `FStar.GSet.equal` 
+      FStar.GSet.singleton (ghost_map_empty `ghost_map_union` ghost_map_empty, l)
+    );
+    assert (
+      ((map_group_zero_or_one (map_group_match_item key value) `map_group_concat` bound_map_group l (map_group_filter p)) l) `FStar.GSet.equal`
+      (map_group_filter p l)
+    )
+  | Some (ll, (k, v), lr) ->
+    let l1 = (ghost_map_singleton k v, ll `List.Tot.append` lr) in
+    assert (map_group_match_item_witness_pred key value l l1 (ll, (k, v), lr));
+    assert (FStar.GSet.mem l1 (map_group_match_item key value l));
+    assert (~ (map_group_match_item key value l == FStar.GSet.empty));
+    map_group_concat_bound_map_group_elim (map_group_zero_or_one (map_group_match_item key value)) (map_group_filter p) l l (fun _ -> ());
+    map_group_zero_or_one_match_item_filter key value p
+
+#restart-solver
+let map_group_zero_or_more_match_item_filter (key value: typ) : Lemma
+  (ensures
+    map_group_zero_or_more (map_group_match_item key value) == map_group_filter (notp (FStar.Ghost.Pull.pull (matches_map_group_entry key value)))
+  )
+= let f = (notp (FStar.Ghost.Pull.pull (matches_map_group_entry key value))) in
+  map_group_equiv_intro_equiv_rec
+    (map_group_zero_or_more (map_group_match_item key value))
+    (map_group_filter (notp (FStar.Ghost.Pull.pull (matches_map_group_entry key value))))
+    (fun l prf l' ->
+      map_group_zero_or_more_zero_or_one_eq (map_group_match_item key value);
+      map_group_zero_or_more_eq (map_group_zero_or_one (map_group_match_item key value)) l;
+      assert (~ (map_group_zero_or_one (map_group_match_item key value) l == FStar.GSet.empty));
+      Classical.forall_intro prf;
+      bound_map_group_ext l (map_group_zero_or_more (map_group_match_item key value)) (map_group_filter f);
+      map_group_zero_or_one_bound_match_item_filter key value l
+    )
 
 #restart-solver
 let apply_map_group_det_zero_or_more_match_item
@@ -1226,54 +1827,15 @@ let apply_map_group_det_zero_or_more_match_item
   (apply_map_group_det (map_group_zero_or_more (map_group_match_item key value)) l ==
     MapGroupDet (List.Tot.filter (notp (FStar.Ghost.Pull.pull (matches_map_group_entry key value))) l)
   )
-= map_group_zero_or_more_match_item_eq key value l;
-  assert (
-    map_group_zero_or_more (map_group_match_item key value) l ==
-    FStar.GSet.singleton (List.Tot.filter (notp (FStar.Ghost.Pull.pull (matches_map_group_entry key value))) l)
-  )
-
-let map_group_filter
-  f
-= FE.on_dom_g cbor_map #map_group_codom (fun l ->
-    FStar.GSet.singleton (List.Tot.filter f l)
-  )
-
-let apply_map_group_det_filter
-  f l
-= ()
-
-let list_filter_implies_2' (#t: Type) (p1 p2: t -> bool) : Lemma
-  (requires (forall (x: t) . p1 x ==> p2 x))
-  (ensures forall  (l: list t) . List.Tot.filter p1 (List.Tot.filter p2 l) == List.Tot.filter p1 l)
-= Classical.forall_intro (fun l -> Classical.move_requires (list_filter_implies_2 p1 p2) l)
-
-#restart-solver
-let map_group_zero_or_one_match_item_filter
-  key value p
-= map_group_equiv_intro
-    (map_group_zero_or_one (map_group_match_item key value) `map_group_concat` map_group_filter p)
-    (map_group_filter p)
-    (fun l l' ->
-      let l1 = map_group_concat_elim (map_group_zero_or_one (map_group_match_item key value)) (map_group_filter p) l l' in
-      if FStar.StrongExcludedMiddle.strong_excluded_middle (map_group_match_item key value l == FStar.GSet.empty)
-      then ()
-      else begin
-        let (ll, kv, lr) = map_group_match_item_elim key value l l1 in
-        list_filter_append p ll (kv :: lr);
-        list_filter_append p ll lr
-      end
-    )
-    (fun l l' ->
-      if not (FStar.StrongExcludedMiddle.strong_excluded_middle (exists l1 . FStar.GSet.mem l1 (map_group_match_item key value l)))
-      then assert (map_group_match_item key value l `FStar.GSet.equal` FStar.GSet.empty)
-      else begin
-        let l1 = FStar.IndefiniteDescription.indefinite_description_ghost _ (fun l1 -> FStar.GSet.mem l1 (map_group_match_item key value l)) in
-        let (ll, kv, lr) = map_group_match_item_elim key value l l1 in
-        list_filter_append p ll (kv :: lr);
-        list_filter_append p ll lr;
-        assert (l' == List.Tot.filter p l1);
-        assert (gset_collect_witness_pred (map_group_filter p) (apply_map_group (map_group_zero_or_one (map_group_match_item key value)) l) l' l1)
-      end
+= map_group_zero_or_more_match_item_filter key value;
+  ghost_map_filter_ext
+    (matches_map_group_entry key value)
+    (notp (notp (FStar.Ghost.Pull.pull (matches_map_group_entry key value))))
+    (ghost_map_of_list l);
+  apply_map_group_det_eq_singleton (map_group_zero_or_more (map_group_match_item key value)) l
+    (
+      ghost_map_filter (matches_map_group_entry key value) (ghost_map_of_list l),
+      List.Tot.filter (notp (FStar.Ghost.Pull.pull (matches_map_group_entry key value))) l
     )
 
 let rec list_filter_and_extract_none
@@ -1326,7 +1888,16 @@ let map_group_zero_or_one_choice
 = map_group_choice_assoc g1 g2 map_group_nop
 
 let matches_map_group (g: map_group) (m: cbor_map) : GTot bool =
-    FStar.GSet.mem [] (g m)
+  FStar.StrongExcludedMiddle.strong_excluded_middle (exists gm .
+    FStar.GSet.mem (gm, []) (g m)
+  )
+
+let matches_map_group_mem (g: map_group) (m: cbor_map) (gm: _) : Lemma
+  (requires FStar.GSet.mem (gm, []) (g m))
+  (ensures gm == ghost_map_of_list m)
+  [SMTPat (FStar.GSet.mem (gm, []) (g m))]
+= Classical.forall_intro (ghost_map_of_list_mem m);
+  ghost_map_equiv gm (ghost_map_of_list m)
 
 let matches_map_group_det (g: map_group) (m: cbor_map) : Lemma
   (match apply_map_group_det g m with
@@ -1335,13 +1906,29 @@ let matches_map_group_det (g: map_group) (m: cbor_map) : Lemma
   | _ -> True)
 = ()
 
+let map_group_entry_consumed_prop
+  (l: cbor_map)
+  (entry: (Cbor.raw_data_item & Cbor.raw_data_item))
+  (g: map_group)
+  l'
+: Tot prop
+= FStar.GSet.mem l' (g l) /\ ghost_map_mem entry (fst l')
+
 let map_group_entry_consumed
   (l: cbor_map)
   (entry: (Cbor.raw_data_item & Cbor.raw_data_item))
   (g: map_group)
 : Tot prop
-= List.Tot.memP entry l /\
-  (exists l' . FStar.GSet.mem l' (g l) /\ ~ (List.Tot.memP entry l'))
+= exists l' . map_group_entry_consumed_prop l entry g l'
+
+let map_group_entry_consumed_elim
+  (l: cbor_map)
+  (entry: (Cbor.raw_data_item & Cbor.raw_data_item))
+  (g: map_group)
+: Ghost _
+    (requires (map_group_entry_consumed l entry g))
+    (ensures fun l' -> map_group_entry_consumed_prop l entry g l')
+= FStar.IndefiniteDescription.indefinite_description_ghost _ (fun l' -> map_group_entry_consumed_prop l entry g l')
 
 let map_group_entry_consumed_matches_map_group
   (l: cbor_map)
@@ -1360,9 +1947,11 @@ let map_group_entry_consumed_concat
   (requires map_group_entry_consumed l entry (g1 `map_group_concat` g2))
   (ensures
     map_group_entry_consumed l entry g1 \/
-    (exists l' . FStar.GSet.mem l' (apply_map_group g1 l) /\ map_group_entry_consumed l' entry g2)
+    (exists l' . FStar.GSet.mem l' (g1 l) /\ map_group_entry_consumed (snd l') entry g2)
   )
-= ()
+= let l' = map_group_entry_consumed_elim l entry (g1 `map_group_concat` g2) in
+  let (l1, l2) = map_group_concat_elim g1 g2 l l' in
+  ()
 
 let map_group_entry_consumed_concat_det
   (l: cbor_map)
@@ -1376,7 +1965,7 @@ let map_group_entry_consumed_concat_det
     map_group_entry_consumed l entry g1 \/
     (let MapGroupDet l' = apply_map_group_det g1 l in map_group_entry_consumed l' entry g2)
   )
-= ()
+= map_group_entry_consumed_concat l entry g1 g2
 
 let map_group_entry_consumed_match_item_intro
   (l: cbor_map)
@@ -1391,16 +1980,8 @@ let map_group_entry_consumed_match_item_intro
     map_group_entry_consumed l kv (map_group_match_item key value)
   )
 = let (ll, lr) = list_memP_extract kv l in
-  assert (map_group_match_item_witness_pred key value l (ll `List.Tot.append` lr) (ll, kv, lr));
-  List.Tot.map_append fst ll (kv :: lr);
-  List.Tot.no_repeats_p_append (List.Tot.map fst ll) (List.Tot.map fst (kv :: lr));
-  assert (~ (List.Tot.memP (fst kv) (List.Tot.map fst ll)));
-  assert (~ (List.Tot.memP (fst kv) (List.Tot.map fst lr)));
-  List.Tot.append_memP (List.Tot.map fst ll) (List.Tot.map fst lr) (fst kv);
-  List.Tot.map_append fst ll lr;
-  assert (~ (List.Tot.memP (fst kv) (List.Tot.map fst (ll `List.Tot.append` lr))));
-  Classical.move_requires (List.Tot.memP_map_intro fst kv) (ll `List.Tot.append` lr);
-  assert (~ (List.Tot.memP kv (ll `List.Tot.append` lr)))
+  let (k, v) = kv in
+  assert (map_group_match_item_witness_pred key value l (ghost_map_singleton k v, ll `List.Tot.append` lr) (ll, kv, lr))
 
 let map_group_entry_consumed_match_item_elim
   (l: cbor_map)
@@ -1414,11 +1995,7 @@ let map_group_entry_consumed_match_item_elim
     List.Tot.memP kv l /\
     matches_map_group_entry key value kv
   )
-= let l' = FStar.IndefiniteDescription.indefinite_description_ghost _ (fun l' -> FStar.GSet.mem l' (map_group_match_item key value l) /\ ~ (List.Tot.memP kv l')) in
-  let (ll, kv', lr) = map_group_match_item_elim key value l l' in
-  List.Tot.append_memP ll lr kv;
-  List.Tot.append_memP ll (kv' :: lr) kv;
-  assert (kv == kv')
+= ()
 
 let map_group_entry_consumed_match_item
   (l: cbor_map)
